theories/program_logic/sim/proofmode.v
@@ -11,17 +11,17 @@ From simuliris.program_logic Require Export
 From simuliris.program_logic Require Import
   sim.notations.
 
-Section sim_state.
+Section sim.
   Context `{!BiBUpd PROP, !BiAffine PROP}.
   Context `{sim_state : !SimState PROP Λₛ Λₜ}.
-  Context (progₛ : program Λₛ) (progₜ : program Λₜ).
+  Context `{sim_programs : !SimPrograms Λₛ Λₜ}.
   Context (X : sim_protocol PROP Λₛ Λₜ).
 
   #[global] Instance frame_simv p R eₛ eₜ Φ1 Φ2 :
     (∀ eₛ eₜ, Frame p R (Φ1 eₛ eₜ) (Φ2 eₛ eₜ)) →
     Frame p R
-      (SIM progₛ; eₛ ≳ progₜ; eₜ [[ X ]] [[ Φ1 ]])
-      (SIM progₛ; eₛ ≳ progₜ; eₜ [[ X ]] [[ Φ2 ]]).
+      (SIM eₛ ≳ eₜ [[ X ]] [[ Φ1 ]])
+      (SIM eₛ ≳ eₜ [[ X ]] [[ Φ2 ]]).
   Proof.
     rewrite /Frame simv_frame_l.
     iIntros "%HR Hsim".
@@ -30,8 +30,8 @@ Section sim_state.
 
   #[global] Instance elim_modal_cupd_simv p P eₛ eₜ Φ :
     ElimModal True p false (|++> P) P
-      (SIM progₛ; eₛ ≳ progₜ; eₜ [[ X ]] [[ Φ ]])
-      (SIM progₛ; eₛ ≳ progₜ; eₜ [[ X ]] [[ Φ ]]).
+      (SIM eₛ ≳ eₜ [[ X ]] [[ Φ ]])
+      (SIM eₛ ≳ eₜ [[ X ]] [[ Φ ]]).
   Proof.
     rewrite /ElimModal bi.intuitionistically_if_elim.
     iIntros "_ (HP & Hsim)".
@@ -39,8 +39,8 @@ Section sim_state.
   Qed.
   #[global] Instance elim_modal_bupd_simv p P eₛ eₜ Φ :
     ElimModal True p false (|==> P) P
-      (SIM progₛ; eₛ ≳ progₜ; eₜ [[ X ]] [[ Φ ]])
-      (SIM progₛ; eₛ ≳ progₜ; eₜ [[ X ]] [[ Φ ]]).
+      (SIM eₛ ≳ eₜ [[ X ]] [[ Φ ]])
+      (SIM eₛ ≳ eₜ [[ X ]] [[ Φ ]]).
   Proof.
     rewrite /ElimModal bi.intuitionistically_if_elim.
     iIntros "_ (HP & Hsim)".
@@ -48,14 +48,14 @@ Section sim_state.
   Qed.
 
   #[global] Instance add_modal_cupd_simv P eₛ eₜ Φ :
-    AddModal (|++> P) P (SIM progₛ; eₛ ≳ progₜ; eₜ [[ X ]] [[ Φ ]]).
+    AddModal (|++> P) P (SIM eₛ ≳ eₜ [[ X ]] [[ Φ ]]).
   Proof.
     rewrite /AddModal.
     iIntros "(HP & Hsim)".
     iApply cupd_simv. iMod "HP". iApply ("Hsim" with "HP").
   Qed.
   #[global] Instance add_modal_bupd_simv P eₛ eₜ Φ :
-    AddModal (|==> P) P (SIM progₛ; eₛ ≳ progₜ; eₜ [[ X ]] [[ Φ ]]).
+    AddModal (|==> P) P (SIM eₛ ≳ eₜ [[ X ]] [[ Φ ]]).
   Proof.
     rewrite /AddModal.
     iIntros "(HP & Hsim)".
@@ -65,16 +65,16 @@ Section sim_state.
   Lemma tac_simv_eval eₛ eₛ' eₜ eₜ' Φ Δ :
     (∀ (eₛ'' := eₛ'), eₛ = eₛ'') →
     (∀ (eₜ'' := eₜ'), eₜ = eₜ'') →
-    envs_entails Δ (SIM progₛ; eₛ' ≳ progₜ; eₜ' [[ X ]] [[ Φ ]]) →
-    envs_entails Δ (SIM progₛ; eₛ ≳ progₜ; eₜ [[ X ]] [[ Φ ]]).
+    envs_entails Δ (SIM eₛ' ≳ eₜ' [[ X ]] [[ Φ ]]) →
+    envs_entails Δ (SIM eₛ ≳ eₜ [[ X ]] [[ Φ ]]).
   Proof.
     intros -> ->. done.
   Qed.
 
   Lemma tac_simv_strongly_stuck eₛ eₜ Φ Δ :
-    IsStronglyStuck progₛ eₛ →
-    IsStronglyStuck progₜ eₜ →
-    envs_entails Δ (SIM progₛ; eₛ ≳ progₜ; eₜ [[ X ]] [[ Φ ]]).
+    IsStronglyStuck sim_progₛ eₛ →
+    IsStronglyStuck sim_progₜ eₜ →
+    envs_entails Δ (SIM eₛ ≳ eₜ [[ X ]] [[ Φ ]]).
   Proof.
     rewrite envs_entails_unseal.
     iIntros. iApply simv_strongly_stuck; done.
@@ -84,37 +84,37 @@ Section sim_state.
     eₛ = of_val vₛ →
     eₜ = of_val vₜ →
     envs_entails Δ (Φ vₛ vₜ) →
-    envs_entails Δ (SIM progₛ; eₛ ≳ progₜ; eₜ [[ X ]] [[ Φ ]]).
+    envs_entails Δ (SIM eₛ ≳ eₜ [[ X ]] [[ Φ ]]).
   Proof.
     rewrite envs_entails_unseal => -> -> ->.
     iIntros. iApply simv_post; done.
   Qed.
 
   Lemma tac_cupd_simv eₛ eₜ Φ Δ :
-    envs_entails Δ (|++> SIM progₛ; eₛ ≳ progₜ; eₜ [[ X ]] [[ Φ ]]) →
-    envs_entails Δ (SIM progₛ; eₛ ≳ progₜ; eₜ [[ X ]] [[ Φ ]]).
+    envs_entails Δ (|++> SIM eₛ ≳ eₜ [[ X ]] [[ Φ ]]) →
+    envs_entails Δ (SIM eₛ ≳ eₜ [[ X ]] [[ Φ ]]).
   Proof.
     rewrite envs_entails_unseal => ->.
     iApply cupd_simv.
   Qed.
   Lemma tac_bupd_simv eₛ eₜ Φ Δ :
-    envs_entails Δ (|==> SIM progₛ; eₛ ≳ progₜ; eₜ [[ X ]] [[ Φ ]]) →
-    envs_entails Δ (SIM progₛ; eₛ ≳ progₜ; eₜ [[ X ]] [[ Φ ]]).
+    envs_entails Δ (|==> SIM eₛ ≳ eₜ [[ X ]] [[ Φ ]]) →
+    envs_entails Δ (SIM eₛ ≳ eₜ [[ X ]] [[ Φ ]]).
   Proof.
     rewrite envs_entails_unseal => ->.
     iApply bupd_simv.
   Qed.
 
   Lemma tac_simv_cupd eₛ eₜ Φ Δ :
-    envs_entails Δ (SIM progₛ; eₛ ≳ progₜ; eₜ [[ X ]] [[ λ eₛ eₜ, |++> Φ eₛ eₜ ]]) →
-    envs_entails Δ (SIM progₛ; eₛ ≳ progₜ; eₜ [[ X ]] [[ Φ ]]).
+    envs_entails Δ (SIM eₛ ≳ eₜ [[ X ]] [[ λ eₛ eₜ, |++> Φ eₛ eₜ ]]) →
+    envs_entails Δ (SIM eₛ ≳ eₜ [[ X ]] [[ Φ ]]).
   Proof.
     rewrite envs_entails_unseal => ->.
     iApply simv_cupd.
   Qed.
   Lemma tac_simv_bupd eₛ eₜ Φ Δ :
-    envs_entails Δ (SIM progₛ; eₛ ≳ progₜ; eₜ [[ X ]] [[ λ eₛ eₜ, |==> Φ eₛ eₜ ]]) →
-    envs_entails Δ (SIM progₛ; eₛ ≳ progₜ; eₜ [[ X ]] [[ Φ ]]).
+    envs_entails Δ (SIM eₛ ≳ eₜ [[ X ]] [[ λ eₛ eₜ, |==> Φ eₛ eₜ ]]) →
+    envs_entails Δ (SIM eₛ ≳ eₜ [[ X ]] [[ Φ ]]).
   Proof.
     rewrite envs_entails_unseal => ->.
     iApply simv_bupd.
@@ -124,12 +124,12 @@ Section sim_state.
     fₛ = (λ vₛ, Kₛ @@ vₛ) →
     fₜ = (λ vₜ, Kₜ @@ vₜ) →
     envs_entails Δ (
-      SIM progₛ; eₛ ≳ progₜ; eₜ [[ X ]] [[ λ vₛ vₜ,
-        SIM progₛ; fₛ (of_val vₛ) ≳ progₜ; fₜ (of_val vₜ) [[ X ]] [[ Φ ]]
+      SIM eₛ ≳ eₜ [[ X ]] [[ λ vₛ vₜ,
+        SIM fₛ (of_val vₛ) ≳ fₜ (of_val vₜ) [[ X ]] [[ Φ ]]
       ]]
     ) →
     envs_entails Δ (
-      SIM progₛ; Kₛ @@ eₛ ≳ progₜ; Kₜ @@ eₜ [[ X ]] [[ Φ ]]
+      SIM Kₛ @@ eₛ ≳ Kₜ @@ eₜ [[ X ]] [[ Φ ]]
     ).
   Proof.
     rewrite envs_entails_unseal -simv_bind => -> -> -> //.
@@ -137,12 +137,12 @@ Section sim_state.
   Lemma tac_simv_bindₛ K f eₛ eₜ Φ Δ :
     f = (λ vₛ, K @@ vₛ) →
     envs_entails Δ (
-      SIM progₛ; eₛ ≳ progₜ; eₜ [[ X ]] [[ λ vₛ vₜ,
-        SIM progₛ; f (of_val vₛ) ≳ progₜ; of_val vₜ [[ X ]] [[ Φ ]]
+      SIM eₛ ≳ eₜ [[ X ]] [[ λ vₛ vₜ,
+        SIM f (of_val vₛ) ≳ of_val vₜ [[ X ]] [[ Φ ]]
       ]]
     ) →
     envs_entails Δ (
-      SIM progₛ; K @@ eₛ ≳ progₜ; eₜ [[ X ]] [[ Φ ]]
+      SIM K @@ eₛ ≳ eₜ [[ X ]] [[ Φ ]]
     ).
   Proof.
     rewrite envs_entails_unseal -simv_bindₛ => -> -> //.
@@ -150,38 +150,38 @@ Section sim_state.
   Lemma tac_simv_bindₜ eₛ K f eₜ Φ Δ :
     f = (λ eₜ, K @@ eₜ) →
     envs_entails Δ (
-      SIM progₛ; eₛ ≳ progₜ; eₜ [[ X ]] [[ λ vₛ vₜ,
-        SIM progₛ; of_val vₛ ≳ progₜ; f (of_val vₜ) [[ X ]] [[ Φ ]]
+      SIM eₛ ≳ eₜ [[ X ]] [[ λ vₛ vₜ,
+        SIM of_val vₛ ≳ f (of_val vₜ) [[ X ]] [[ Φ ]]
       ]]
     ) →
     envs_entails Δ (
-      SIM progₛ; eₛ ≳ progₜ; K @@ eₜ [[ X ]] [[ Φ ]]
+      SIM eₛ ≳ K @@ eₜ [[ X ]] [[ Φ ]]
     ).
   Proof.
     rewrite envs_entails_unseal -simv_bindₜ => -> -> //.
   Qed.
 
   Lemma tac_simv_pure_execₛ ϕ n K eₛ1 eₛ2 eₜ Φ Δ :
-    PureExec progₛ ϕ n eₛ1 eₛ2 →
+    PureExec sim_progₛ ϕ n eₛ1 eₛ2 →
     ϕ →
-    envs_entails Δ (SIM progₛ; K @@ eₛ2 ≳ progₜ; eₜ [[ X ]] [[ Φ ]]) →
-    envs_entails Δ (SIM progₛ; K @@ eₛ1 ≳ progₜ; eₜ [[ X ]] [[ Φ ]]).
+    envs_entails Δ (SIM K @@ eₛ2 ≳ eₜ [[ X ]] [[ Φ ]]) →
+    envs_entails Δ (SIM K @@ eₛ1 ≳ eₜ [[ X ]] [[ Φ ]]).
   Proof.
     pose proof @pure_exec_fill_pure_exec.
     rewrite envs_entails_unseal => ? ? ->.
     eapply simv_pure_stepsₛ, rtc_nsteps_2, pure_exec; done.
   Qed.
   Lemma tac_simv_pure_execₜ ϕ n eₛ K eₜ1 eₜ2 Φ Δ :
-    PureExec progₜ ϕ n eₜ1 eₜ2 →
+    PureExec sim_progₜ ϕ n eₜ1 eₜ2 →
     ϕ →
-    envs_entails Δ (SIM progₛ; eₛ ≳ progₜ; K @@ eₜ2 [[ X ]] [[ Φ ]]) →
-    envs_entails Δ (SIM progₛ; eₛ ≳ progₜ; K @@ eₜ1 [[ X ]] [[ Φ ]]).
+    envs_entails Δ (SIM eₛ ≳ K @@ eₜ2 [[ X ]] [[ Φ ]]) →
+    envs_entails Δ (SIM eₛ ≳ K @@ eₜ1 [[ X ]] [[ Φ ]]).
   Proof.
     pose proof @pure_exec_fill_pure_exec.
     rewrite envs_entails_unseal => ? ? ->.
     eapply simv_pure_stepsₜ, rtc_nsteps_2, pure_exec; done.
   Qed.
-End sim_state.
+End sim.
 
 Tactic Notation "expr_is_val" open_constr(e) :=
   eunify (of_val _) e.
@@ -193,8 +193,8 @@ Tactic Notation "ectx_is_empty" open_constr(K) :=
 Tactic Notation "match_simv" tactic3(tac_succ) tactic3(tac_fail) :=
   iStartProof;
   lazymatch goal with
-  | |- envs_entails ?Δ (simv ?progₛ ?progₜ ?X ?Φ ?eₛ ?eₜ) =>
-      tac_succ Δ progₛ progₜ X Φ eₛ eₜ
+  | |- envs_entails ?Δ (simv ?X ?Φ ?eₛ ?eₜ) =>
+      tac_succ Δ X Φ eₛ eₜ
   | _ =>
       tac_fail ()
   end.
@@ -203,8 +203,8 @@ Tactic Notation "on_simv" tactic3(tac) :=
   match_simv ltac:(tac) ltac:(fun _ => fail "not a 'simv'").
 
 Tactic Notation "simv_eval" tactic3(tacₛ) tactic3(tacₜ) :=
-  on_simv ltac:(fun _ _ _ _ _ _ _ =>
-    notypeclasses refine (tac_simv_eval _ _ _ _ _ _ _ _ _ _ _ _);
+  on_simv ltac:(fun _ _ _ _ _ =>
+    notypeclasses refine (tac_simv_eval _ _ _ _ _ _ _ _ _ _);
     [ let x := fresh in intros x; tacₛ; unfold x; notypeclasses refine eq_refl
     | let x := fresh in intros x; tacₜ; unfold x; notypeclasses refine eq_refl
     | idtac
@@ -225,17 +225,13 @@ Ltac simv_simplₜ :=
   simv_evalₜ simpl.
 
 Ltac simv_simpl_post :=
-  iStartProof;
-  lazymatch goal with
-  | |- envs_entails ?Δ (simv ?progₛ ?progₜ ?X ?Φ ?eₛ ?eₜ) =>
-      let Φ := eval simpl in Φ in
-      change (envs_entails Δ (simv progₛ progₜ X Φ eₛ eₜ))
-  | _ =>
-     fail "simv_simpl_post: not a 'simv'"
-  end.
+  on_simv ltac:(fun Δ X Φ eₛ eₜ =>
+    let Φ := eval simpl in Φ in
+    change (envs_entails Δ (simv X Φ eₛ eₜ))
+  ).
 
 Ltac simv_strongly_stuck :=
-  on_simv ltac:(fun _ _ _ _ _ _ _ =>
+  on_simv ltac:(fun _ _ _ _ _ =>
     eapply tac_simv_strongly_stuck;
     [ iSolveTC
     | iSolveTC
@@ -243,16 +239,16 @@ Ltac simv_strongly_stuck :=
   ).
 
 Ltac cupd_sim :=
-  on_simv ltac:(fun _ _ _ _ _ _ _ =>
+  on_simv ltac:(fun _ _ _ _ _ =>
     eapply tac_cupd_simv
   ).
 
 Ltac simv_cupd_simple :=
-  on_simv ltac:(fun _ _ _ _ _ _ _ =>
+  on_simv ltac:(fun _ _ _ _ _ =>
     eapply tac_simv_cupd
   ).
 Ltac simv_cupd :=
-  on_simv ltac:(fun _ _ _ _ Φ _ _ =>
+  on_simv ltac:(fun _ _ Φ _ _ =>
     first
     [ assert (∀ P eₛ eₜ, AddModal (|++> P) P (Φ eₛ eₜ)) as _ by iSolveTC
     | simv_cupd_simple
@@ -260,16 +256,16 @@ Ltac simv_cupd :=
   ).
 
 Ltac bupd_sim :=
-  on_simv ltac:(fun _ _ _ _ _ _ _ =>
+  on_simv ltac:(fun _ _ _ _ _ =>
     eapply tac_bupd_simv
   ).
 
 Ltac simv_bupd_simple :=
-  on_simv ltac:(fun _ _ _ _ _ _ _ =>
+  on_simv ltac:(fun _ _ _ _ _ =>
     eapply tac_simv_bupd
   ).
 Ltac simv_bupd :=
-  on_simv ltac:(fun _ _ _ _ Φ _ _ =>
+  on_simv ltac:(fun _ _ Φ _ _ =>
     first
     [ assert (∀ P eₛ eₜ, AddModal (|==> P) P (Φ eₛ eₜ)) as _ by iSolveTC
     | simv_bupd_simple
@@ -277,7 +273,7 @@ Ltac simv_bupd :=
   ).
 
 Ltac simv_post_simple :=
-  on_simv ltac:(fun _ _ _ _ _ _ _ =>
+  on_simv ltac:(fun _ _ _ _ _ =>
     eapply tac_simv_post;
     [ reflexivity
     | reflexivity
@@ -301,7 +297,7 @@ Tactic Notation "simv_bind_coreₛ" open_constr(K) :=
   tryif ectx_is_empty K then (
     idtac
   ) else (
-    eapply (tac_simv_bindₛ _ _ _ K);
+    eapply (tac_simv_bindₛ _ K);
     [ simpl; reflexivity
     | pm_prettify; simv_simpl_post
     ]
@@ -310,7 +306,7 @@ Tactic Notation "simv_bind_coreₜ" open_constr(K) :=
   tryif ectx_is_empty K then (
     idtac
   ) else (
-    eapply (tac_simv_bindₜ _ _ _ _ K);
+    eapply (tac_simv_bindₜ _ _ K);
     [ simpl; reflexivity
     | pm_prettify; simv_simpl_post
     ]
@@ -322,7 +318,7 @@ Tactic Notation "simv_bind_core" open_constr(Kₛ) open_constr(Kₜ) :=
     tryif ectx_is_empty Kₜ then (
       simv_bind_coreₛ Kₛ
     ) else (
-      eapply (tac_simv_bind _ _ _ Kₛ _ _ Kₜ);
+      eapply (tac_simv_bind _ Kₛ _ _ Kₜ);
       [ simpl; reflexivity
       | simpl; reflexivity
       | pm_prettify; simv_simpl_post
@@ -331,7 +327,7 @@ Tactic Notation "simv_bind_core" open_constr(Kₛ) open_constr(Kₜ) :=
   ).
 
 Tactic Notation "simv_pure_coreₛ" open_constr(K) "with" tactic3(tac) :=
-  eapply (tac_simv_pure_execₛ _ _ _ _ _ K);
+  eapply (tac_simv_pure_execₛ _ _ _ K);
   [ iSolveTC
   | try done
   | simv_finish with tac
@@ -339,7 +335,7 @@ Tactic Notation "simv_pure_coreₛ" open_constr(K) "with" tactic3(tac) :=
 Tactic Notation "simv_pure_coreₛ" open_constr(K) :=
   simv_pure_coreₛ K with idtac.
 Tactic Notation "simv_pure_coreₜ" open_constr(K) "with" tactic3(tac) :=
-  eapply (tac_simv_pure_execₜ _ _ _ _ _ _ K);
+  eapply (tac_simv_pure_execₜ _ _ _ _ K);
   [ iSolveTC
   | try done
   | simv_finish with tac
