theories/tmc/sim/derived_rules.v
@@ -6,9 +6,9 @@ From simuliris.tmc Require Import
   sim.proofmode
   sim.notations.
 
-Section sim_GS.
+Section sim.
+  Context `{sim_programs : !SimPrograms ectx_language ectx_language}.
   Context `{sim_GS : !SimGS Σ}.
-  Context (progₛ progₜ : program).
   Context (X : sim_protocol Σ).
   Implicit Types func : function.
   Implicit Types constr : constructor.
@@ -18,12 +18,12 @@ Section sim_GS.
   Implicit Types Φ : val → val → iProp Σ.
 
   Lemma simv_let eₛ1 eₛ2 eₜ1 eₜ2 Φ :
-    SIM progₛ; eₛ1 ≳ progₜ; eₜ1 [[ X ]] [[ (≈) ]] -∗
+    SIM eₛ1 ≳ eₜ1 [[ X ]] [[ (≈) ]] -∗
     ( ∀ vₛ vₜ,
       vₛ ≈ vₜ -∗
-      SIM progₛ; eₛ2.[#vₛ/] ≳ progₜ; eₜ2.[#vₜ/] [[ X ]] [[ Φ ]]
+      SIM eₛ2.[#vₛ/] ≳ eₜ2.[#vₜ/] [[ X ]] [[ Φ ]]
     ) -∗
-    SIM progₛ; let: eₛ1 in eₛ2 ≳ progₜ; let: eₜ1 in eₜ2 [[ X ]] [[ Φ ]].
+    SIM let: eₛ1 in eₛ2 ≳ let: eₜ1 in eₜ2 [[ X ]] [[ Φ ]].
   Proof.
     iIntros "Hsim1 Hsim2".
     simv_mono "Hsim1". iIntros "%vₛ %vₜ #Hv".
@@ -32,25 +32,25 @@ Section sim_GS.
 
   Lemma simv_call eₛ1 eₛ2 eₜ1 eₜ2 Φ :
     ( ∀ func vₛ vₜ,
-      Func func ≈ Func func -∗
+      ⌜func ∈ dom sim_progₛ⌝ -∗
       vₛ ≈ vₜ -∗
-      SIM progₛ; func vₛ ≳ progₜ; func vₜ [[ X ]] [[ Φ ]]
+      SIM func vₛ ≳ func vₜ [[ X ]] [[ Φ ]]
     ) -∗
-    SIM progₛ; eₛ1 ≳ progₜ; eₜ1 [[ X ]] [[ (≈) ]] -∗
-    SIM progₛ; eₛ2 ≳ progₜ; eₜ2 [[ X ]] [[ (≈) ]] -∗
-    SIM progₛ; eₛ1 eₛ2 ≳ progₜ; eₜ1 eₜ2 [[ X ]] [[ Φ ]].
+    SIM eₛ1 ≳ eₜ1 [[ X ]] [[ (≈) ]] -∗
+    SIM eₛ2 ≳ eₜ2 [[ X ]] [[ (≈) ]] -∗
+    SIM eₛ1 eₛ2 ≳ eₜ1 eₜ2 [[ X ]] [[ Φ ]].
   Proof.
     iIntros "Hsim Hsim1 Hsim2".
     simv_mono "Hsim2". iIntros "%vₛ2 %vₜ2 #Hv2".
     simv_mono "Hsim1". iIntros "%vₛ1 %vₜ1 #Hv1".
     destruct vₛ1, vₜ1; try iDestruct "Hv1" as %[]; try simv_strongly_stuck.
-    simv_apply ("Hsim" with "[//] Hv2").
+    subst. simv_apply ("Hsim" with "[//] Hv2").
   Qed.
 
   Lemma simv_unop op eₛ eₜ Φ :
-    SIM progₛ; eₛ ≳ progₜ; eₜ [[ X ]] [[ (≈) ]] -∗
+    SIM eₛ ≳ eₜ [[ X ]] [[ (≈) ]] -∗
     (∀ vₛ vₜ, vₛ ≈ vₜ -∗ Φ vₛ vₜ) -∗
-    SIM progₛ; Unop op eₛ ≳ progₜ; Unop op eₜ [[ X ]] [[ Φ ]].
+    SIM Unop op eₛ ≳ Unop op eₜ [[ X ]] [[ Φ ]].
   Proof.
     iIntros "Hsim HΦ".
     simv_mono "Hsim". iIntros "%vₛ %vₜ #Hv".
@@ -61,10 +61,10 @@ Section sim_GS.
   Qed.
 
   Lemma simv_binop op eₛ1 eₛ2 eₜ1 eₜ2 Φ :
-    SIM progₛ; eₛ1 ≳ progₜ; eₜ1 [[ X ]] [[ (≈) ]] -∗
-    SIM progₛ; eₛ2 ≳ progₜ; eₜ2 [[ X ]] [[ (≈) ]] -∗
+    SIM eₛ1 ≳ eₜ1 [[ X ]] [[ (≈) ]] -∗
+    SIM eₛ2 ≳ eₜ2 [[ X ]] [[ (≈) ]] -∗
     (∀ vₛ vₜ, vₛ ≈ vₜ -∗ Φ vₛ vₜ) -∗
-    SIM progₛ; Binop op eₛ1 eₛ2 ≳ progₜ; Binop op eₜ1 eₜ2 [[ X ]] [[ Φ ]].
+    SIM Binop op eₛ1 eₛ2 ≳ Binop op eₜ1 eₜ2 [[ X ]] [[ Φ ]].
   Proof.
     iIntros "Hsim1 Hsim2 HΦ".
     simv_mono "Hsim2". iIntros "%vₛ2 %vₜ2 #Hv2".
@@ -73,14 +73,14 @@ Section sim_GS.
     destruct vₛ2, vₜ2; try iDestruct "Hv2" as %[];
     destruct op; try simv_strongly_stuck;
       simv_pures;
-      iApply "HΦ"; auto.
+      iApply "HΦ"; subst; auto.
   Qed.
 
   Lemma simv_if eₛ0 eₛ1 eₛ2 eₜ0 eₜ1 eₜ2 Φ :
-    SIM progₛ; eₛ0 ≳ progₜ; eₜ0 [[ X ]] [[ (≈) ]] -∗
-    SIM progₛ; eₛ1 ≳ progₜ; eₜ1 [[ X ]] [[ Φ ]] -∗
-    SIM progₛ; eₛ2 ≳ progₜ; eₜ2 [[ X ]] [[ Φ ]] -∗
-    SIM progₛ; If eₛ0 eₛ1 eₛ2 ≳ progₜ; If eₜ0 eₜ1 eₜ2 [[ X ]] [[ Φ ]].
+    SIM eₛ0 ≳ eₜ0 [[ X ]] [[ (≈) ]] -∗
+    SIM eₛ1 ≳ eₜ1 [[ X ]] [[ Φ ]] -∗
+    SIM eₛ2 ≳ eₜ2 [[ X ]] [[ Φ ]] -∗
+    SIM If eₛ0 eₛ1 eₛ2 ≳ If eₜ0 eₜ1 eₜ2 [[ X ]] [[ Φ ]].
   Proof.
     iIntros "Hsim0 Hsim1 Hsim2".
     simv_mono "Hsim0". iIntros "%vₛ0 %vₜ0 #Hv0".
@@ -89,10 +89,10 @@ Section sim_GS.
   Qed.
 
   Lemma simv_constr constr eₛ1 eₛ2 eₜ1 eₜ2 Φ :
-    SIM progₛ; eₛ1 ≳ progₜ; eₜ1 [[ X ]] [[ (≈) ]] -∗
-    SIM progₛ; eₛ2 ≳ progₜ; eₜ2 [[ X ]] [[ (≈) ]] -∗
+    SIM eₛ1 ≳ eₜ1 [[ X ]] [[ (≈) ]] -∗
+    SIM eₛ2 ≳ eₜ2 [[ X ]] [[ (≈) ]] -∗
     (∀ lₛ lₜ, Loc lₛ ≈ Loc lₜ -∗ Φ lₛ lₜ) -∗
-    SIM progₛ; &constr eₛ1 eₛ2 ≳ progₜ; &constr eₜ1 eₜ2 [[ X ]] [[ Φ ]].
+    SIM &constr eₛ1 eₛ2 ≳ &constr eₜ1 eₜ2 [[ X ]] [[ Φ ]].
   Proof.
     iIntros "Hsim1 Hsim2 HΦ".
     simv_constrₜ;
@@ -104,7 +104,7 @@ Section sim_GS.
       iApply "HΦ"; done.
   Qed.
   Lemma simv_constr_valₜ1 eₛ constr eₜ vₜ2 Φ :
-    SIM progₛ; eₛ ≳ progₜ; eₜ [[ X ]] [[ (≈) ]] -∗
+    SIM eₛ ≳ eₜ [[ X ]] [[ (≈) ]] -∗
     ( ∀ vₛ l vₜ1,
       (l +ₗ 0) ↦ₜ constr -∗
       (l +ₗ 1) ↦ₜ vₜ1 -∗
@@ -112,7 +112,7 @@ Section sim_GS.
       vₛ ≈ vₜ1 -∗
       Φ vₛ l
     ) -∗
-    SIM progₛ; eₛ ≳ progₜ; &constr eₜ vₜ2 [[ X ]] [[ Φ ]].
+    SIM eₛ ≳ &constr eₜ vₜ2 [[ X ]] [[ Φ ]].
   Proof.
     iIntros "Hsim HΦ".
     simv_constrₜ;
@@ -121,7 +121,7 @@ Section sim_GS.
       iApply ("HΦ" with "Hl0 Hl1 Hl2 Hv").
   Qed.
   Lemma simv_constr_valₜ2 eₛ constr vₜ1 eₜ Φ :
-    SIM progₛ; eₛ ≳ progₜ; eₜ [[ X ]] [[ (≈) ]] -∗
+    SIM eₛ ≳ eₜ [[ X ]] [[ (≈) ]] -∗
     ( ∀ vₛ l vₜ2,
       (l +ₗ 0) ↦ₜ constr -∗
       (l +ₗ 1) ↦ₜ vₜ1 -∗
@@ -129,7 +129,7 @@ Section sim_GS.
       vₛ ≈ vₜ2 -∗
       Φ vₛ l
     ) -∗
-    SIM progₛ; eₛ ≳ progₜ; &constr vₜ1 eₜ [[ X ]] [[ Φ ]].
+    SIM eₛ ≳ &constr vₜ1 eₜ [[ X ]] [[ Φ ]].
   Proof.
     iIntros "Hsim HΦ".
     simv_constrₜ;
@@ -139,10 +139,10 @@ Section sim_GS.
   Qed.
 
   Lemma simv_load eₛ1 eₛ2 eₜ1 eₜ2 Φ :
-    SIM progₛ; eₛ1 ≳ progₜ; eₜ1 [[ X ]] [[ (≈) ]] -∗
-    SIM progₛ; eₛ2 ≳ progₜ; eₜ2 [[ X ]] [[ (≈) ]] -∗
+    SIM eₛ1 ≳ eₜ1 [[ X ]] [[ (≈) ]] -∗
+    SIM eₛ2 ≳ eₜ2 [[ X ]] [[ (≈) ]] -∗
     (∀ vₛ vₜ, vₛ ≈ vₜ -∗ Φ vₛ vₜ) -∗
-    SIM progₛ; ![eₛ2] eₛ1 ≳ progₜ; ![eₜ2] eₜ1 [[ X ]] [[ Φ ]].
+    SIM ![eₛ2] eₛ1 ≳ ![eₜ2] eₜ1 [[ X ]] [[ Φ ]].
   Proof.
     iIntros "Hsim1 Hsim2 HΦ".
     simv_mono "Hsim2". iIntros "%vₛ2 %vₜ2 #Hv2".
@@ -155,11 +155,11 @@ Section sim_GS.
   Qed.
 
   Lemma simv_store eₛ1 eₛ2 eₛ3 eₜ1 eₜ2 eₜ3 Φ :
-    SIM progₛ; eₛ1 ≳ progₜ; eₜ1 [[ X ]] [[ (≈) ]] -∗
-    SIM progₛ; eₛ2 ≳ progₜ; eₜ2 [[ X ]] [[ (≈) ]] -∗
-    SIM progₛ; eₛ3 ≳ progₜ; eₜ3 [[ X ]] [[ (≈) ]] -∗
+    SIM eₛ1 ≳ eₜ1 [[ X ]] [[ (≈) ]] -∗
+    SIM eₛ2 ≳ eₜ2 [[ X ]] [[ (≈) ]] -∗
+    SIM eₛ3 ≳ eₜ3 [[ X ]] [[ (≈) ]] -∗
     Φ ()%V ()%V -∗
-    SIM progₛ; eₛ1 <-[eₛ2]- eₛ3 ≳ progₜ; eₜ1 <-[eₜ2]- eₜ3 [[ X ]] [[ Φ ]].
+    SIM eₛ1 <-[eₛ2]- eₛ3 ≳ eₜ1 <-[eₜ2]- eₜ3 [[ X ]] [[ Φ ]].
   Proof.
     iIntros "Hsim1 Hsim2 Hsim3 HΦ".
     simv_mono "Hsim3". iIntros "%vₛ3 %vₜ3 #Hv3".
@@ -170,4 +170,4 @@ Section sim_GS.
       try simv_strongly_stuck.
     simv_store.
   Qed.
-End sim_GS.
+End sim.
